Protocols/RB/Protocol.v
@@ -118,6 +118,12 @@ Definition th_echo4ready := N - t0.
 Definition th_ready4ready := N - (t0 + t0).
 Definition th_ready4output := N - t0.
 
+Fact th_echo4ready_gt_0 : 0 < th_echo4ready.
+Proof. unfold th_echo4ready. pose proof t0_lt_N. lia. Qed.
+
+Fact th_ready4ready_gt_0 : 0 < th_ready4ready.
+Proof. unfold th_ready4ready. pose proof t0_lt_N_minus_2t0. lia. Qed.
+
 Definition check_ready_condition (st : State) (msg : Message) : bool :=
   let: Node n smap emap vmap cnt omap := st in
   match msg with
